o Finished proving some result regarding diff_abs_bot.

computation/computation_preserves_diff_abs_bot.v
@@ -92,6 +92,23 @@ Ltac inv_diff_imp :=
       assert (diff_abs_bot_b b3 b4) as h2 by (apply H; auto);
       assert (diff_abs_bot_b b5 b6) as h3 by (apply H; auto);
       clear H
+  | [ H : forall _ _ : _, (?b1,?b2) = _ [+] (?b3,?b4) = _ [+] (?b5,?b6) = _ [+] (?b7,?b8) = _ [+] False -> _ |- _ ] =>
+    let h1 := fresh H in
+    let h2 := fresh H in
+    let h3 := fresh H in
+    let h4 := fresh H in
+    assert (diff_abs_bot_b b1 b2) as h1 by (apply H; auto);
+      assert (diff_abs_bot_b b3 b4) as h2 by (apply H; auto);
+      assert (diff_abs_bot_b b5 b6) as h3 by (apply H; auto);
+      assert (diff_abs_bot_b b7 b8) as h4 by (apply H; auto);
+      clear H
+  | [ H : forall _ _ : _, (?b1,?b2) = _ [+] LIn _ (combine ?bs1 ?bs2) -> _ |- _ ] =>
+    let h1 := fresh H in
+    let h2 := fresh H in
+    let i  := fresh "i" in
+    assert (diff_abs_bot_b b1 b2) as h1 by (apply H; auto);
+      assert (forall b1 b2, LIn (b1,b2) (combine bs1 bs2) -> diff_abs_bot_b b1 b2) as h2 by (introv i; apply H; auto);
+      clear H
   | [ H : forall _ _ : _, (?b1,?b2) = _ [+] (?b3,?b4) = _ [+] LIn _ (combine ?bs1 ?bs2) -> _ |- _ ] =>
     let h1 := fresh H in
     let h2 := fresh H in
@@ -100,6 +117,30 @@ Ltac inv_diff_imp :=
     assert (diff_abs_bot_b b1 b2) as h1 by (apply H; auto);
       assert (diff_abs_bot_b b3 b4) as h2 by (apply H; auto);
       assert (forall b1 b2, LIn (b1,b2) (combine bs1 bs2) -> diff_abs_bot_b b1 b2) as h3 by (introv i; apply H; auto);
+      clear H
+  | [ H : forall _ _ : _, (?b1,?b2) = _ [+] (?b3,?b4) = _ [+] (?b5,?b6) = _ [+] LIn _ (combine ?bs1 ?bs2) -> _ |- _ ] =>
+    let h1 := fresh H in
+    let h2 := fresh H in
+    let h3 := fresh H in
+    let h4 := fresh H in
+    let i  := fresh "i" in
+    assert (diff_abs_bot_b b1 b2) as h1 by (apply H; auto);
+      assert (diff_abs_bot_b b3 b4) as h2 by (apply H; auto);
+      assert (diff_abs_bot_b b5 b6) as h3 by (apply H; auto);
+      assert (forall b1 b2, LIn (b1,b2) (combine bs1 bs2) -> diff_abs_bot_b b1 b2) as h4 by (introv i; apply H; auto);
+      clear H
+  | [ H : forall _ _ : _, (?b1,?b2) = _ [+] (?b3,?b4) = _ [+] (?b5,?b6) = _ [+] (?b7,?b8) = _ [+] LIn _ (combine ?bs1 ?bs2) -> _ |- _ ] =>
+    let h1 := fresh H in
+    let h2 := fresh H in
+    let h3 := fresh H in
+    let h4 := fresh H in
+    let h5 := fresh H in
+    let i  := fresh "i" in
+    assert (diff_abs_bot_b b1 b2) as h1 by (apply H; auto);
+      assert (diff_abs_bot_b b3 b4) as h2 by (apply H; auto);
+      assert (diff_abs_bot_b b5 b6) as h3 by (apply H; auto);
+      assert (diff_abs_bot_b b7 b8) as h4 by (apply H; auto);
+      assert (forall b1 b2, LIn (b1,b2) (combine bs1 bs2) -> diff_abs_bot_b b1 b2) as h5 by (introv i; apply H; auto);
       clear H
   end.
 
@@ -175,6 +216,91 @@ Proof.
 Qed.
 Hint Resolve diff_abs_bot_alpha_eapply : slow.
 
+Lemma implies_alpha_eq_mk_exception {o} :
+  forall (a1 a2 b1 b2 : @NTerm o),
+    alpha_eq a1 b1
+    -> alpha_eq a2 b2
+    -> alpha_eq (mk_exception a1 a2) (mk_exception b1 b2).
+Proof.
+  introv aeq1 aeq2.
+  apply alpha_eq_oterm_combine; simpl; dands; auto.
+  introv i; repndors; tcsp; ginv; apply alphaeqbt_nilv2; auto.
+Qed.
+
+Lemma diff_abs_bot_alpha_exc {o} :
+  forall (a b c d : @NTerm o),
+    diff_abs_bot_alpha a c
+    -> diff_abs_bot_alpha b d
+    -> diff_abs_bot_alpha (mk_exception a b) (mk_exception c d).
+Proof.
+  introv d1 d2.
+  allunfold @diff_abs_bot_alpha; exrepnd.
+  eexists; eexists; dands;
+  try (apply implies_alpha_eq_mk_exception);
+  try eassumption.
+  constructor; simpl; auto.
+  introv i; repndors; ginv; tcsp; constructor; auto.
+Qed.
+Hint Resolve diff_abs_bot_alpha_exc : slow.
+
+Lemma implies_alpha_eq_mk_arithop {o} :
+  forall op (a1 a2 b1 b2 : @NTerm o),
+    alpha_eq a1 b1
+    -> alpha_eq a2 b2
+    -> alpha_eq (mk_arithop op a1 a2) (mk_arithop op b1 b2).
+Proof.
+  introv aeq1 aeq2.
+  apply alpha_eq_oterm_combine; simpl; dands; auto.
+  introv i; repndors; tcsp; ginv; apply alphaeqbt_nilv2; auto.
+Qed.
+
+Lemma implies_alpha_eq_mk_compop {o} :
+  forall op (a1 a2 a3 a4 b1 b2 b3 b4 : @NTerm o),
+    alpha_eq a1 b1
+    -> alpha_eq a2 b2
+    -> alpha_eq a3 b3
+    -> alpha_eq a4 b4
+    -> alpha_eq (mk_compop op a1 a2 a3 a4) (mk_compop op b1 b2 b3 b4).
+Proof.
+  introv aeq1 aeq2 aeq3 aeq4.
+  apply alpha_eq_oterm_combine; simpl; dands; auto.
+  introv i; repndors; tcsp; ginv; apply alphaeqbt_nilv2; auto.
+Qed.
+
+Lemma diff_abs_bot_alpha_arithop {o} :
+  forall op (a b c d : @NTerm o),
+    diff_abs_bot_alpha a c
+    -> diff_abs_bot_alpha b d
+    -> diff_abs_bot_alpha (mk_arithop op a b) (mk_arithop op c d).
+Proof.
+  introv d1 d2.
+  allunfold @diff_abs_bot_alpha; exrepnd.
+  eexists; eexists; dands;
+  try (apply implies_alpha_eq_mk_arithop);
+  try eassumption.
+  constructor; simpl; auto.
+  introv i; repndors; ginv; tcsp; constructor; auto.
+Qed.
+Hint Resolve diff_abs_bot_alpha_arithop : slow.
+
+Lemma diff_abs_bot_alpha_compop {o} :
+  forall op (a1 a2 a3 a4 b1 b2 b3 b4 : @NTerm o),
+    diff_abs_bot_alpha a1 b1
+    -> diff_abs_bot_alpha a2 b2
+    -> diff_abs_bot_alpha a3 b3
+    -> diff_abs_bot_alpha a4 b4
+    -> diff_abs_bot_alpha (mk_compop op a1 a2 a3 a4) (mk_compop op b1 b2 b3 b4).
+Proof.
+  introv d1 d2 d3 d4.
+  allunfold @diff_abs_bot_alpha; exrepnd.
+  eexists; eexists; dands;
+  try (apply implies_alpha_eq_mk_compop);
+  try eassumption.
+  constructor; simpl; auto.
+  introv i; repndors; ginv; tcsp; constructor; auto.
+Qed.
+Hint Resolve diff_abs_bot_alpha_compop : slow.
+
 Lemma diff_abs_bot_alpha_apply {o} :
   forall (a b c d : @NTerm o),
     diff_abs_bot_alpha a c
@@ -191,6 +317,24 @@ Proof.
 Qed.
 Hint Resolve diff_abs_bot_alpha_apply : slow.
 
+Lemma diff_abs_bot_alpha_atom_eq {o} :
+  forall (a1 a2 a3 a4 b1 b2 b3 b4 : @NTerm o),
+    diff_abs_bot_alpha a1 b1
+    -> diff_abs_bot_alpha a2 b2
+    -> diff_abs_bot_alpha a3 b3
+    -> diff_abs_bot_alpha a4 b4
+    -> diff_abs_bot_alpha (mk_atom_eq a1 a2 a3 a4) (mk_atom_eq b1 b2 b3 b4).
+Proof.
+  introv d1 d2 d3 d4.
+  allunfold @diff_abs_bot_alpha; exrepnd.
+  eexists; eexists; dands;
+  try (apply implies_alpha_eq_mk_atom_eq);
+  try eassumption.
+  constructor; simpl; auto.
+  introv i; repndors; ginv; tcsp; constructor; auto.
+Qed.
+Hint Resolve diff_abs_bot_alpha_atom_eq : slow.
+
 Lemma diff_abs_bot_alpha_fix {o} :
   forall (a b : @NTerm o),
     diff_abs_bot_alpha a b
@@ -206,6 +350,21 @@ Proof.
 Qed.
 Hint Resolve diff_abs_bot_alpha_fix : slow.
 
+Lemma diff_abs_bot_alpha_fresh {o} :
+  forall v (a b : @NTerm o),
+    diff_abs_bot_alpha a b
+    -> diff_abs_bot_alpha (mk_fresh v a) (mk_fresh v b).
+Proof.
+  introv d.
+  allunfold @diff_abs_bot_alpha; exrepnd.
+  eexists; eexists; dands;
+  try (apply implies_alpha_eq_mk_fresh);
+  try eassumption.
+  constructor; simpl; auto.
+  introv i; repndors; ginv; tcsp; constructor; auto.
+Qed.
+Hint Resolve diff_abs_bot_alpha_fresh : slow.
+
 Lemma diff_abs_bot_preserves_isnoncan_like {o} :
   forall (t1 t2 : @NTerm o),
     isnoncan_like t1
@@ -216,6 +375,17 @@ Proof.
   inversion d; subst; try (unfold mk_vbot, mk_bottom, mk_fix); auto.
 Qed.
 Hint Resolve diff_abs_bot_preserves_isnoncan_like : slow.
+
+Lemma diff_abs_bot_preserves_isvalue_like {o} :
+  forall (t1 t2 : @NTerm o),
+    isvalue_like t1
+    -> diff_abs_bot t1 t2
+    -> isvalue_like t2.
+Proof.
+  introv isn d.
+  inversion d; subst; try (unfold mk_vbot, mk_bottom, mk_fix); auto.
+Qed.
+Hint Resolve diff_abs_bot_preserves_isvalue_like : slow.
 
 Lemma diff_abs_bot_sym {o} :
   forall (t1 t2 : @NTerm o),
@@ -505,9 +675,7 @@ Proof.
     inversion p0; subst; auto.
 Qed.
 
-XXXXXXXXXXXXXX
-
-Lemma diff_abs_bot_lsubst {o} :
+Lemma diff_abs_bot_alpha_lsubst {o} :
   forall (t1 t2 : @NTerm o) sub1 sub2,
     diff_abs_bot t1 t2
     -> diff_abs_bot_subs sub1 sub2
@@ -515,37 +683,553 @@ Lemma diff_abs_bot_lsubst {o} :
 Proof.
   introv d1 d2.
 
-  pose proof (change_bvars_alpha_wspec (sub_free_vars sub1) t1) as h.
-  destruct h as [t1' h]; repnd.
+  pose proof (diff_abs_bot_change_bound_vars
+                (sub_free_vars sub1 ++ sub_free_vars sub2)
+                t1 t2 d1) as h.
+  exrepnd.
 
-  pose proof (change_bvars_alpha_wspec (sub_free_vars sub2) t2) as q.
-  destruct q as [t2' q]; repnd.
+  eapply diff_abs_bot_alpha_l;[apply lsubst_alpha_congr2;exact h2|].
+  eapply diff_abs_bot_alpha_r;[|apply alpha_eq_sym;apply lsubst_alpha_congr2;exact h3].
+  clear dependent t1.
+  clear dependent t2.
+  allrw disjoint_app_r; repnd.
 
-  eapply diff_abs_bot_alpha_l;[apply lsubst_alpha_congr2;exact h|].
-  eapply diff_abs_bot_alpha_r;[|apply alpha_eq_sym;apply lsubst_alpha_congr2;exact q].
-
-  pose proof (unfold_lsubst sub1 t1') as z; exrepnd.
+  pose proof (unfold_lsubst sub1 u1) as z; exrepnd.
   rewrite z0; clear z0.
 
-  pose proof (unfold_lsubst sub2 t2) as q; exrepnd.
+  pose proof (unfold_lsubst sub2 u2) as q; exrepnd.
   rewrite q0; clear q0.
 
-  exists (lsubst_aux t1 sub1) (lsubst_aux t2 sub2).
+  exists (lsubst_aux u1 sub1) (lsubst_aux u2 sub2).
 
+  dands; try (apply lsubst_aux_alpha_congr_same_disj); eauto 3 with slow.
   apply diff_abs_bot_lsubst_aux; auto.
+Qed.
 
+Lemma diff_abs_bot_preserves_isexc {o} :
+  forall (t1 t2 : @NTerm o),
+    diff_abs_bot t1 t2
+    -> isexc t1
+    -> isexc t2.
+Proof.
+  introv d ise.
+  apply isexc_implies2 in ise; exrepnd; subst.
+  invdiff.
+Qed.
+Hint Resolve diff_abs_bot_preserves_isexc : slow.
+
+Lemma diff_abs_bot_preserves_eapply_wf_def {o} :
+  forall can (bs1 bs2 : list (@BTerm o)),
+    eapply_wf_def (oterm (Can can) bs1)
+    -> length bs1 = length bs2
+    -> (forall b1 b2, LIn (b1, b2) (combine bs1 bs2) -> diff_abs_bot_b b1 b2)
+    -> eapply_wf_def (oterm (Can can) bs2).
+Proof.
+  introv w e i.
+  allunfold @eapply_wf_def; repndors; exrepnd; subst;
+  allunfold @mk_nseq; allunfold @mk_lam; ginv; allsimpl; cpx; tcsp.
+  - right; left; eexists; eauto.
+  - allsimpl; inv_diff_imp; invdiff.
+    right; right.
+    eexists; eexists; eauto.
+Qed.
+Hint Resolve diff_abs_bot_preserves_eapply_wf_def : slow.
+
+Lemma hasvalue_like_eapply_can_right {o} :
+  forall lib (a b : @NTerm o),
+    iscan a
+    -> hasvalue_like lib (mk_eapply a b)
+    -> hasvalue_like lib b.
+Proof.
+  introv isc hv.
+  allunfold @hasvalue_like; exrepnd.
+  allunfold @reduces_to; exrepnd.
+  revert dependent b.
+  induction k; introv comp.
+
+  - allrw @reduces_in_atmost_k_steps_0; subst.
+    unfold isvalue_like in *; allsimpl; tcsp.
+
+  - allrw @reduces_in_atmost_k_steps_S; exrepnd.
+    csunf comp1; allsimpl.
+    destruct a as [x|g|op bs]; ginv.
+
+    + apply compute_step_eapply_success in comp1; exrepnd; ginv.
+      repndors; exrepnd.
+
+      * apply compute_step_eapply2_success in comp1; repnd; GC.
+        repndors; exrepnd; subst; ginv.
+        exists (@mk_nat o n); dands; eauto 3 with slow.
+        exists 0.
+        apply reduces_in_atmost_k_steps_0; auto.
+
+      * subst.
+        apply isexc_implies2 in comp2; exrepnd; subst; ginv.
+        exists (oterm Exc l); dands; eauto 3 with slow.
+        exists 0.
+        apply reduces_in_atmost_k_steps_0; auto.
+
+      * subst.
+        apply IHk in comp0; exrepnd.
+        exists v0; dands; auto.
+        exists (S k0).
+        apply reduces_in_atmost_k_steps_S.
+        eexists; dands; eauto.
+
+    + apply iscan_implies in isc; repndors; exrepnd; ginv.
+      apply compute_step_eapply_success in comp1; exrepnd; ginv.
+      repndors; exrepnd.
+
+      * apply compute_step_eapply2_success in comp1; repnd; GC.
+        exists arg2; dands; eauto 3 with slow.
+        exists 0.
+        apply reduces_in_atmost_k_steps_0; auto.
+
+      * subst.
+        exists arg2; dands; eauto 3 with slow.
+        exists 0.
+        apply reduces_in_atmost_k_steps_0; auto.
+
+      * subst.
+        apply IHk in comp0; exrepnd.
+        exists v0; dands; auto.
+        exists (S k0).
+        apply reduces_in_atmost_k_steps_S.
+        eexists; dands; eauto.
+Qed.
+Hint Resolve hasvalue_like_eapply_can_right : slow.
+
+Lemma hasvalue_like_eapply_sterm_right {o} :
+  forall lib f (a : @NTerm o),
+    hasvalue_like lib (mk_eapply (sterm f) a)
+    -> hasvalue_like lib a.
+Proof.
+  introv hv.
+  apply hasvalue_like_eapply_can_right in hv; eauto 3 with slow.
+Qed.
+Hint Resolve hasvalue_like_eapply_sterm_right : slow.
+
+Lemma hasvalue_like_arithop_can_right {o} :
+  forall lib c (a b : @NTerm o),
+    iscan a
+    -> hasvalue_like lib (mk_arithop c a b)
+    -> hasvalue_like lib b.
+Proof.
+  introv isc hv.
+  allunfold @hasvalue_like; exrepnd.
+  allunfold @reduces_to; exrepnd.
+  revert dependent b.
+  induction k; introv comp.
+
+  - allrw @reduces_in_atmost_k_steps_0; subst.
+    unfold isvalue_like in *; allsimpl; tcsp.
+
+  - allrw @reduces_in_atmost_k_steps_S; exrepnd.
+    apply iscan_implies in isc; repndors; exrepnd; subst.
+
+    + apply compute_step_narithop_can1_success in comp1.
+      repnd; repndors; exrepnd; ginv.
+
+      * apply compute_step_arithop_success_can_can in comp3; exrepnd; subst; GC.
+        exists (oterm (Can can') []); dands; eauto 3 with slow.
+        exists 0.
+        apply reduces_in_atmost_k_steps_0; auto.
+
+      * subst; allunfold @nobnd; ginv.
+        apply IHk in comp0; exrepnd.
+        exists v0; dands; auto.
+        exists (S k0).
+        apply reduces_in_atmost_k_steps_S.
+        eexists; dands; eauto.
+
+      * exists t; dands; eauto 3 with slow.
+        exists 0.
+        apply reduces_in_atmost_k_steps_0; auto.
+
+    + csunf comp1; allsimpl; ginv.
+Qed.
+Hint Resolve hasvalue_like_arithop_can_right : slow.
+
+Lemma hasvalue_like_compop_can_right {o} :
+  forall lib co (a b c d : @NTerm o),
+    iscan a
+    -> hasvalue_like lib (mk_compop co a b c d)
+    -> hasvalue_like lib b.
+Proof.
+  introv isc hv.
+  allunfold @hasvalue_like; exrepnd.
+  allunfold @reduces_to; exrepnd.
+  revert dependent b.
+  induction k; introv comp.
+
+  - allrw @reduces_in_atmost_k_steps_0; subst.
+    unfold isvalue_like in *; allsimpl; tcsp.
+
+  - allrw @reduces_in_atmost_k_steps_S; exrepnd.
+    apply iscan_implies in isc; repndors; exrepnd; subst.
+
+    + apply compute_step_ncompop_can1_success in comp1.
+      repnd; repndors; exrepnd; ginv.
+
+      * apply compute_step_compop_success_can_can in comp3; exrepnd; subst; GC.
+        exists (oterm (Can can') []); dands; eauto 3 with slow.
+        exists 0.
+        apply reduces_in_atmost_k_steps_0; auto.
+
+      * subst; allunfold @nobnd; ginv.
+        apply IHk in comp0; exrepnd.
+        exists v0; dands; auto.
+        exists (S k0).
+        apply reduces_in_atmost_k_steps_S.
+        eexists; dands; eauto.
+
+      * exists t; dands; eauto 3 with slow.
+        exists 0.
+        apply reduces_in_atmost_k_steps_0; auto.
+
+    + csunf comp1; allsimpl; ginv.
+Qed.
+Hint Resolve hasvalue_like_compop_can_right : slow.
+
+Lemma not_hasvalue_like_vbot {o} :
+  forall lib v, !@hasvalue_like o lib (mk_vbot v).
+Proof.
+  introv hv.
+  unfold hasvalue_like in hv; exrepnd.
+  apply reduces_to_vbot_if_isvalue_like in hv1; auto.
+Qed.
+
+Lemma hasvalue_like_compute_step {o} :
+  forall lib (t u : @NTerm o),
+    hasvalue_like lib t
+    -> compute_step lib t = csuccess u
+    -> hasvalue_like lib u.
+Proof.
+  introv hv comp.
+  allunfold @hasvalue_like; exrepnd.
+  apply reduces_to_split2 in hv1; repndors; exrepnd; subst.
+  - rewrite compute_step_value_like in comp; auto; ginv.
+    exists u; dands; auto.
+    apply reduces_to_symm.
+  - rewrite hv1 in comp; ginv.
+    exists v; dands; auto.
+Qed.
+
+Lemma hasvalue_like_ncan_fst {o} :
+  forall lib ncan (t : @NTerm o) bs,
+    hasvalue_like lib (oterm (NCan ncan) (bterm [] t :: bs))
+    -> hasvalue_like lib t.
+Proof.
+  introv hv.
+  allunfold @hasvalue_like; exrepnd.
+  pose proof (converges_to_value_like_ncan lib ncan t bs) as h.
+  autodimp h hyp.
+
+  {
+    unfold converges_to_value_like.
+    exists v; dands; auto.
+  }
+
+  exrepnd.
+  exists u; dands; repndors; eauto 3 with slow.
+Qed.
+
+Definition diff_abs_bot_b_alpha {o} (b1 b2 : @BTerm o) :=
+  {u1 : BTerm
+   & {u2 : BTerm
+   & alpha_eq_bterm b1 u1
+   # alpha_eq_bterm b2 u2
+   # diff_abs_bot_b u1 u2}}.
+
+Definition diff_abs_bot_bs_alpha {o} (bs1 bs2 : list (@BTerm o)) :=
+  br_bterms diff_abs_bot_b_alpha bs1 bs2.
+
+Lemma diff_abs_bot_bterms_cons {o} :
+  forall (b1 b2 : @BTerm o) bs1 bs2,
+    diff_abs_bot_bterms (b1 :: bs1) (b2 :: bs2)
+    <=> (diff_abs_bot_b b1 b2 # diff_abs_bot_bterms bs1 bs2).
+Proof.
+  unfold diff_abs_bot_bterms; introv.
+  rw @br_bterms_cons_iff; sp.
+Qed.
+
+Lemma diff_abs_bot_bterms_nil {o} :
+  @diff_abs_bot_bterms o [] [].
+Proof.
+  unfold diff_abs_bot_bterms, br_bterms, br_list; simpl; sp.
+Qed.
+Hint Resolve diff_abs_bot_bterms_nil : slow.
+
+Lemma diff_abs_bot_bterms_cons_if {o} :
+  forall (b1 b2 : @BTerm o) bs1 bs2,
+    diff_abs_bot_b b1 b2
+    -> diff_abs_bot_bterms bs1 bs2
+    -> diff_abs_bot_bterms (b1 :: bs1) (b2 :: bs2).
+Proof.
+  introv d1 d2; apply diff_abs_bot_bterms_cons; sp.
+Qed.
+Hint Resolve diff_abs_bot_bterms_cons_if : slow.
+
+Lemma diff_abs_bot_bs_alpha_cons {o} :
+  forall (b1 b2 : @BTerm o) bs1 bs2,
+    diff_abs_bot_bs_alpha (b1 :: bs1) (b2 :: bs2)
+    <=> (diff_abs_bot_b_alpha b1 b2 # diff_abs_bot_bs_alpha bs1 bs2).
+Proof.
+  unfold diff_abs_bot_bs_alpha; introv.
+  rw @br_bterms_cons_iff; sp.
+Qed.
+
+Lemma diff_abs_bot_bs_alpha_cons_if {o} :
+  forall (b1 b2 : @BTerm o) bs1 bs2,
+    diff_abs_bot_b_alpha b1 b2
+    -> diff_abs_bot_bs_alpha bs1 bs2
+    -> diff_abs_bot_bs_alpha (b1 :: bs1) (b2 :: bs2).
+Proof.
+  introv d1 d2; apply diff_abs_bot_bs_alpha_cons; sp.
+Qed.
+Hint Resolve diff_abs_bot_bs_alpha_cons_if : slow.
+
+Lemma diff_abs_bot_b_implies_diff_abs_bot_b_alpha {o} :
+  forall (b1 b2 : @BTerm o),
+    diff_abs_bot_b b1 b2
+    -> diff_abs_bot_b_alpha b1 b2.
+Proof.
+  introv d.
+  exists b1 b2; dands; eauto 3 with slow.
+Qed.
+Hint Resolve diff_abs_bot_b_implies_diff_abs_bot_b_alpha : slow.
+
+Lemma diff_abs_bot_bterms_implies_diff_abs_bot_bs_alpha {o} :
+  forall (bs1 bs2 : list (@BTerm o)),
+    diff_abs_bot_bterms bs1 bs2
+    -> diff_abs_bot_bs_alpha bs1 bs2.
+Proof.
+  introv d.
+  unfold diff_abs_bot_bterms in d.
+  unfold diff_abs_bot_bs_alpha.
+  allunfold @br_bterms.
+  allunfold @br_list; repnd; dands; auto.
+  introv i; apply d in i.
+  eauto 3 with slow.
+Qed.
+Hint Resolve diff_abs_bot_bterms_implies_diff_abs_bot_bs_alpha : slow.
+
+Lemma implies_diff_abs_bot_alpha_oterm {o} :
+  forall op (bs1 bs2 : list (@BTerm o)),
+    diff_abs_bot_bs_alpha bs1 bs2
+    -> diff_abs_bot_alpha (oterm op bs1) (oterm op bs2).
+Proof.
+  introv diff.
+  unfold diff_abs_bot_bs_alpha, br_bterms, br_list in diff; repnd.
+
+  assert {bs1' : list BTerm
+          & {bs2' : list BTerm
+          & alpha_eq_bterms bs1 bs1'
+          # alpha_eq_bterms bs2 bs2'
+          # diff_abs_bot_bterms bs1' bs2'}} as hbs.
+  { revert dependent bs2.
+    induction bs1; introv len imp; destruct bs2; allsimpl; cpx; GC.
+    - exists ([] : list (@BTerm o)) ([] : list (@BTerm o)); dands; eauto 3 with slow.
+    - pose proof (imp a b) as h; autodimp h hyp.
+      pose proof (IHbs1 bs2) as k; repeat (autodimp k hyp).
+      exrepnd.
+      unfold diff_abs_bot_b_alpha in h; exrepnd.
+      exists (u1 :: bs1') (u2 :: bs2'); dands; eauto 3 with slow. }
+
+  exrepnd.
+  applydup @alpha_eq_bterms_implies_same_length in hbs0.
+  applydup @alpha_eq_bterms_implies_same_length in hbs2.
+  exists (oterm op bs1') (oterm op bs2'); dands; auto.
+
+  - apply alpha_eq_oterm_combine; dands; tcsp.
+    introv i; apply hbs0; auto.
+
+  - apply alpha_eq_oterm_combine; dands; tcsp.
+    introv i; apply hbs2; auto.
+
+  - constructor; try omega.
+    introv i; apply hbs1; auto.
+Qed.
+
+Lemma implies_diff_abs_bot_b_alpha {o} :
+  forall l (t1 t2 : @NTerm o),
+    diff_abs_bot_alpha t1 t2
+    -> diff_abs_bot_b_alpha (bterm l t1) (bterm l t2).
+Proof.
+  introv d.
+  unfold diff_abs_bot_alpha in d; exrepnd.
+  exists (bterm l u1) (bterm l u2); dands; eauto 3 with slow.
+Qed.
+Hint Resolve implies_diff_abs_bot_b_alpha : slow.
+
+Lemma diff_abs_bot_alpha_pushdown_fresh_isvalue_like {o} :
+  forall v (t1 t2 : @NTerm o),
+    isvalue_like t1
+    -> diff_abs_bot t1 t2
+    -> diff_abs_bot_alpha (pushdown_fresh v t1) (pushdown_fresh v t2).
+Proof.
+  introv ivl d.
+  destruct t1 as [v1|f1|op1 bs1]; invdiff; allsimpl; eauto 3 with slow;
+  try (complete (unfold isvalue_like in ivl; allsimpl; tcsp)).
+
+  apply implies_diff_abs_bot_alpha_oterm.
+  unfold diff_abs_bot_bs_alpha, br_bterms, br_list, mk_fresh_bterms.
+  autorewrite with slow; dands; auto.
+  introv i.
+  rewrite <- map_combine in i.
+  apply in_map_iff in i; exrepnd; ginv.
+  applydup imp in i1.
+  destruct a0 as [l1 t1].
+  destruct a as [l2 t2].
+  allsimpl.
+  invdiff.
+  apply implies_diff_abs_bot_b_alpha.
+  unfold maybe_new_var; boolvar; eauto 3 with slow.
+
+  pose proof (ex_fresh_var (all_vars t1 ++ all_vars t2)) as fv; exrepnd.
+  allrw in_app_iff; allrw not_over_or; repnd.
+  exists (mk_fresh v0 t1) (mk_fresh v0 t2).
+  dands; auto.
+
+  { apply (implies_alpha_eq_mk_fresh_sub v0); allrw in_app_iff; tcsp.
+    repeat (rw @lsubst_trivial3); allsimpl; auto.
+    - introv i; repndors; tcsp; cpx; allsimpl; allrw disjoint_singleton_l.
+      dands; auto.
+    - introv i; repndors; tcsp; cpx; allsimpl; allrw disjoint_singleton_l.
+      dands; auto.
+      apply newvar_prop. }
+
+  { apply (implies_alpha_eq_mk_fresh_sub v0); allrw in_app_iff; tcsp.
+    repeat (rw @lsubst_trivial3); allsimpl; auto.
+    - introv i; repndors; tcsp; cpx; allsimpl; allrw disjoint_singleton_l.
+      dands; auto.
+    - introv i; repndors; tcsp; cpx; allsimpl; allrw disjoint_singleton_l.
+      dands; auto.
+      apply newvar_prop. }
+
+  { constructor; auto; simpl.
+    introv i; repndors; cpx. }
+Qed.
+Hint Resolve diff_abs_bot_alpha_pushdown_fresh_isvalue_like : slow.
+
+Hint Resolve get_fresh_atom_prop : slow.
+Hint Rewrite @get_utokens_sub_cons : slow.
+
+Lemma implies_disjoint_singleton_l :
+  forall (A : tuniv) (x : A) (s : list A),
+    !LIn x s
+    -> disjoint [x] s.
+Proof.
+  introv h.
+  apply disjoint_singleton_l; auto.
+Qed.
+Hint Resolve implies_disjoint_singleton_l : slow.
+
+Lemma implies_disjoint_singleton_r :
+  forall (A : tuniv) (x : A) (s : list A),
+    !LIn x s
+    -> disjoint s [x].
+Proof.
+  introv h.
+  apply disjoint_singleton_r; auto.
+Qed.
+Hint Resolve implies_disjoint_singleton_r : slow.
+
+Lemma hasvalue_like_if_compute_step {o} :
+  forall lib (t u : @NTerm o),
+    hasvalue_like lib u
+    -> compute_step lib t = csuccess u
+    -> hasvalue_like lib t.
+Proof.
+  introv hv comp; allunfold @hasvalue_like; exrepnd.
+  exists v; dands; auto.
+  eapply reduces_to_if_split2; eauto.
+Qed.
+
+Lemma diff_abs_bot_subst_utokens_aux {o} :
+  forall (t1 t2 : @NTerm o) sub,
+    diff_abs_bot t1 t2
+    -> diff_abs_bot (subst_utokens_aux t1 sub) (subst_utokens_aux t2 sub).
+Proof.
+  nterm_ind t1 as [v1|f1|op1 bs1 ind1] Case; introv d; invdiff; auto;
+  try (complete (allsimpl; auto));
+  try (complete (allsimpl; constructor)).
+
+  Case "oterm".
+  allrw @subst_utokens_aux_oterm.
+  remember (get_utok op1) as guo1; symmetry in Heqguo1; destruct guo1.
+
+  - unfold subst_utok.
+    remember (utok_sub_find sub g) as sf; symmetry in Heqsf; destruct sf; eauto 3 with slow.
+    constructor; allrw map_length; auto.
+    introv i; allrw <- @map_combine; allrw in_map_iff; exrepnd; cpx; allsimpl.
+    applydup imp in i1; applydup in_combine in i1; repnd.
+    destruct a0 as [l1 u1].
+    destruct a as [l2 u2].
+    invdiff; allsimpl.
+    constructor.
+    eapply ind1; eauto.
+
+  - constructor; allrw map_length; auto.
+    introv i; allrw <- @map_combine; allrw in_map_iff; exrepnd; cpx; allsimpl.
+    applydup imp in i1; applydup in_combine in i1; repnd.
+    destruct a0 as [l1 u1].
+    destruct a as [l2 u2].
+    invdiff; allsimpl.
+    constructor; auto.
+    eapply ind1; eauto.
+Qed.
+
+Lemma diff_abs_bot_alpha_subst_utokens {o} :
+  forall (t1 t2 : @NTerm o) sub,
+    diff_abs_bot_alpha t1 t2
+    -> diff_abs_bot_alpha (subst_utokens t1 sub) (subst_utokens t2 sub).
+Proof.
+  introv d.
+  unfold diff_abs_bot_alpha in d; exrepnd.
+
+  eapply diff_abs_bot_alpha_l;[eapply alpha_eq_subst_utokens_same;exact d0|].
+  eapply diff_abs_bot_alpha_r;[|apply alpha_eq_sym;eapply alpha_eq_subst_utokens_same;exact d2].
+  clear dependent t1.
+  clear dependent t2.
+
+  pose proof (diff_abs_bot_change_bound_vars
+                (free_vars_utok_sub sub)
+                u1 u2 d1) as d; exrepnd.
+  rename u0 into t1.
+  rename u3 into t2.
+
+  eapply diff_abs_bot_alpha_l;[eapply alpha_eq_subst_utokens_same;exact d3|].
+  eapply diff_abs_bot_alpha_r;[|apply alpha_eq_sym;eapply alpha_eq_subst_utokens_same;exact d4].
+  clear dependent u1.
+  clear dependent u2.
+
+  pose proof (unfold_subst_utokens sub t1) as h; exrepnd.
+  pose proof (unfold_subst_utokens sub t2) as k; exrepnd.
+  rename t' into u1.
+  rename t'0 into u2.
+  rw h0; rw k0.
+
+  eapply diff_abs_bot_alpha_l;[apply (alpha_eq_subst_utokens_aux u1 t1 sub sub); eauto 3 with slow|].
+  eapply diff_abs_bot_alpha_r;[|apply alpha_eq_sym;apply (alpha_eq_subst_utokens_aux u2 t2 sub sub); eauto 3 with slow].
+
+  apply diff_abs_bot_implies_alpha.
+  apply diff_abs_bot_subst_utokens_aux; auto.
 Qed.
 
 Lemma compute_step_abs2bot_lsubst_aux {o} :
   forall (t : @NTerm o) t' u,
     wf_term t
+    -> wf_term t'
     -> compute_step [] t = csuccess u
+    (* hasvalue_like is needed in the case where t is bot and t' is abs *)
+    -> hasvalue_like [] u
     -> diff_abs_bot t t'
     -> {u' : NTerm
         & compute_step [] t' = csuccess u'
         # diff_abs_bot_alpha u u'}.
 Proof.
-  nterm_ind1s t as [v|f ind|op bs ind] Case; introv wf comp diff.
+  nterm_ind1s t as [v|f ind|op bs ind] Case; introv wf wf' comp hv diff.
 
   - Case "vterm".
     allsimpl; ginv.
@@ -612,9 +1296,10 @@ Proof.
               pose proof (ind arg2 arg2 []) as h; clear ind.
               repeat (autodimp h hyp); eauto 3 with slow.
               apply wf_term_eapply_iff in wf; exrepnd; allunfold @nobnd; ginv.
-              eapply h in comp1; clear h; auto; try(exact diff).
-              exrepnd; rewrite comp1.
+              apply wf_term_eapply_iff in wf'; exrepnd; allunfold @nobnd; ginv.
               allsimpl; cpx.
+              eapply h in comp1; clear h; auto; try(exact diff); eauto 3 with slow.
+              exrepnd; rewrite comp1.
               eexists; dands; eauto.
               fold_terms; eauto 4 with slow.
           }
@@ -634,21 +1319,23 @@ Proof.
             invdiff.
             csunf; simpl; auto.
             eexists; dands; eauto.
-            eapply alpha_eq_trans;[|apply alpha_eq_sym; apply abs2bot_lsubst]; auto.
+            apply diff_abs_bot_alpha_lsubst; simpl; eauto 3 with slow.
           }
 
           {
             SSCase "NTryCatch".
             apply compute_step_try_success in comp; exrepnd; subst; allsimpl.
+            invdiff.
             csunf; simpl.
-            eexists; dands; eauto.
+            eexists; dands; eauto 7 with slow.
           }
 
           {
             SSCase "NCanTest".
             apply compute_step_seq_can_test_success in comp; exrepnd; subst; allsimpl.
+            invdiff.
             csunf; simpl.
-            eexists; dands; eauto.
+            eexists; dands; eauto 3 with slow.
           }
 
         - dopid op as [can2|ncan2|exc2|abs2] SSCase.
@@ -661,8 +1348,10 @@ Proof.
 
               csunf comp; allsimpl.
               apply compute_step_apply_success in comp.
-              repndors; exrepnd; subst; auto; csunf; simpl; eexists; dands; eauto.
-              eapply alpha_eq_trans;[|apply alpha_eq_sym; apply abs2bot_lsubst]; auto.
+
+              repndors; exrepnd; subst; auto; invdiff;
+              csunf; simpl; eexists; dands; eauto 4 with slow.
+              apply diff_abs_bot_alpha_lsubst; simpl; eauto 3 with slow.
             }
 
             {
@@ -677,31 +1366,38 @@ Proof.
                 repndors; exrepnd; subst; auto; ginv.
 
                 + unfold mk_lam in *; ginv.
+                  invdiff.
                   csunf; simpl.
                   dcwf h; simpl.
                   apply iscan_implies in comp0; repndors; exrepnd; subst; simpl; auto;
+                  invdiff;
                   eexists; dands; eauto;
-                  eapply alpha_eq_trans;
-                  try (apply alpha_eq_sym; apply abs2bot_lsubst); auto.
+                  apply diff_abs_bot_alpha_lsubst; simpl; eauto 3 with slow.
 
                 + unfold mk_nseq in *; allsimpl; ginv; GC.
+                  invdiff.
                   csunf; simpl.
                   dcwf h; simpl.
                   boolvar; simpl; auto; try omega.
                   rewrite Znat.Nat2Z.id; auto.
-                  eexists; dands; eauto.
+                  eexists; dands; eauto 3 with slow.
 
-              - fold_terms; rewrite compute_step_eapply_iscan_isexc; eauto 3 with slow.
+              - invdiff.
+                fold_terms; rewrite compute_step_eapply_iscan_isexc; eauto 3 with slow.
+                eexists; dands; eauto 3 with slow.
 
-              - fold_terms; rewrite compute_step_eapply_iscan_isnoncan_like; eauto 3 with slow.
+              - invdiff.
+                fold_terms; rewrite compute_step_eapply_iscan_isnoncan_like; eauto 3 with slow.
 
                 pose proof (ind arg2 arg2 []) as q; clear ind.
                 repeat (autodimp q hyp); eauto 2 with slow.
                 apply wf_term_eapply_iff in wf; exrepnd; allunfold @nobnd; ginv.
-                apply q in comp1; clear q; auto.
+                apply wf_term_eapply_iff in wf'; exrepnd; allunfold @nobnd; ginv.
+                allsimpl; cpx.
+                eapply q in comp1; clear q; auto; try (exact diff); eauto 3 with slow.
                 exrepnd; rewrite comp1; auto.
                 eexists; dands; eauto.
-                repeat prove_alpha_eq4.
+                apply diff_abs_bot_alpha_eapply; eauto 3 with slow.
             }
 
             {
@@ -710,7 +1406,19 @@ Proof.
               csunf comp; allsimpl.
               apply compute_step_fix_success in comp.
               repndors; exrepnd; subst; auto.
-              csunf; simpl; eexists; dands; eauto.
+              invdiff.
+
+              - csunf; simpl; eexists; dands; eauto.
+                apply diff_abs_bot_alpha_apply; eauto 3 with slow.
+                apply diff_abs_bot_alpha_fix; eauto 3 with slow.
+
+              - fold_terms.
+                eapply hasvalue_like_compute_step in hv;
+                  [|csunf;simpl;auto].
+                unfold apply_bterm in hv; allsimpl.
+                rewrite lsubst_lsubst_aux in hv; allsimpl; auto.
+                boolvar.
+                apply not_hasvalue_like_vbot in hv; tcsp.
             }
 
             {
@@ -719,8 +1427,9 @@ Proof.
               csunf comp; allsimpl.
               apply compute_step_spread_success in comp.
               repndors; exrepnd; subst; auto.
+              invdiff.
               csunf; simpl; eexists; dands; eauto.
-              eapply alpha_eq_trans;[|apply alpha_eq_sym; apply abs2bot_lsubst]; auto.
+              apply diff_abs_bot_alpha_lsubst; simpl; eauto 3 with slow.
             }
 
             {
@@ -729,8 +1438,9 @@ Proof.
               csunf comp; allsimpl.
               apply compute_step_dsup_success in comp.
               repndors; exrepnd; subst; auto.
+              invdiff.
               csunf; simpl; eexists; dands; eauto.
-              eapply alpha_eq_trans;[|apply alpha_eq_sym; apply abs2bot_lsubst]; auto.
+              apply diff_abs_bot_alpha_lsubst; simpl; eauto 3 with slow.
             }
 
             {
@@ -739,10 +1449,11 @@ Proof.
               csunf comp; allsimpl.
               apply compute_step_decide_success in comp.
               repndors; exrepnd; subst; auto.
+              invdiff.
+
               repndors; exrepnd; subst; auto;
               csunf; simpl; eexists; dands; eauto;
-              eapply alpha_eq_trans;
-              try (apply alpha_eq_sym; apply abs2bot_lsubst); auto.
+              apply diff_abs_bot_alpha_lsubst; simpl; eauto 3 with slow.
             }
 
             {
@@ -751,9 +1462,9 @@ Proof.
               csunf comp; allsimpl.
               apply compute_step_cbv_success in comp.
               repndors; exrepnd; subst; auto.
+              invdiff.
               csunf; simpl; eexists; dands; eauto.
-              eapply alpha_eq_trans;
-                try (apply alpha_eq_sym; apply abs2bot_lsubst); auto.
+              apply diff_abs_bot_alpha_lsubst; simpl; eauto 3 with slow.
             }
 
             {
@@ -762,9 +1473,10 @@ Proof.
               csunf comp; allsimpl.
               apply compute_step_sleep_success in comp.
               repndors; exrepnd; subst; auto.
+              invdiff.
               csunf; simpl.
               unfold compute_step_sleep; simpl.
-              eexists; dands; eauto.
+              eexists; dands; eauto 3 with slow.
             }
 
             {
@@ -773,11 +1485,12 @@ Proof.
               csunf comp; allsimpl.
               apply compute_step_tuni_success in comp.
               repndors; exrepnd; subst; auto.
+              invdiff.
               csunf; simpl.
               unfold compute_step_tuni; simpl.
               boolvar; try omega.
               rewrite Znat.Nat2Z.id; auto.
-              eexists; dands; eauto.
+              eexists; dands; eauto 3 with slow.
             }
 
             {
@@ -786,9 +1499,10 @@ Proof.
               csunf comp; allsimpl.
               apply compute_step_minus_success in comp.
               repndors; exrepnd; subst; auto.
+              invdiff.
               csunf; simpl.
               unfold compute_step_minus; simpl.
-              eexists; dands; eauto.
+              eexists; dands; eauto 3 with slow.
             }
 
             {
@@ -803,8 +1517,9 @@ Proof.
               csunf comp; allsimpl.
               apply compute_step_try_success in comp.
               repndors; exrepnd; subst; auto.
+              invdiff.
               csunf; simpl.
-              eexists; dands; eauto.
+              eexists; dands; eauto 7 with slow.
             }
 
             {
@@ -813,71 +1528,82 @@ Proof.
               csunf comp; allsimpl.
               apply compute_step_parallel_success in comp.
               repndors; exrepnd; subst; auto.
+              invdiff.
               csunf; simpl.
               unfold compute_step_parallel.
-              eexists; dands; eauto.
+              eexists; dands; eauto 3 with slow.
             }
 
             {
               SSSCase "NCompOp".
 
               apply compute_step_ncompop_can1_success in comp; repnd.
-              repndors; exrepnd; allsimpl; subst; tcsp; simpl.
+              repndors; exrepnd; allsimpl; subst; tcsp; simpl; invdiff.
 
               - csunf; simpl.
                 dcwf h.
                 apply compute_step_compop_success_can_can in comp1; exrepnd; subst; ginv; GC.
-                repndors; exrepnd; subst; allsimpl;
+
+                repndors; exrepnd; subst; allsimpl; cpx;
                 unfold compute_step_comp; allrw;
                 eexists; dands; eauto;
-                boolvar; auto.
+                boolvar; eauto 3 with slow.
 
               - rewrite compute_step_ncompop_ncanlike2; eauto 3 with slow.
                 dcwf h.
                 pose proof (ind t t []) as q; clear ind.
                 repeat (autodimp q hyp); eauto 2 with slow.
                 allrw @wf_term_ncompop_iff; exrepnd; ginv.
-                apply q in comp4; clear q; auto.
+                allsimpl; cpx.
+                eapply q in comp4; clear q; auto; try (exact diff);
+                try (complete (apply hasvalue_like_compop_can_right in hv; auto)).
                 exrepnd.
                 rewrite comp2; auto.
+                allsimpl; inv_diff_imp; invdiff.
                 eexists; dands; eauto.
-                repeat prove_alpha_eq4.
+                apply diff_abs_bot_alpha_compop; eauto 3 with slow.
 
               - csunf; simpl.
                 apply isexc_implies2 in comp1; exrepnd; subst.
+                invdiff.
                 dcwf h; simpl; auto.
-                eexists; dands; eauto.
+                eexists; dands; eauto 3 with slow.
             }
 
             {
               SSSCase "NArithOp".
 
               apply compute_step_narithop_can1_success in comp; repnd.
-              repndors; exrepnd; allsimpl; subst; tcsp; allsimpl.
+              repndors; exrepnd; allsimpl; subst; tcsp; allsimpl; invdiff.
 
               - csunf; simpl.
                 dcwf h.
                 apply compute_step_arithop_success_can_can in comp1; exrepnd; subst; ginv; GC.
+                allsimpl; cpx.
+
                 repndors; exrepnd; subst; allsimpl;
                 unfold compute_step_comp; allrw;
                 eexists; dands; eauto;
-                boolvar; auto.
+                boolvar; eauto 3 with slow.
 
               - rewrite compute_step_narithop_ncanlike2; eauto 3 with slow.
                 dcwf h.
                 pose proof (ind t t []) as q; clear ind.
                 repeat (autodimp q hyp); eauto 2 with slow.
                 allrw @wf_term_narithop_iff; exrepnd; ginv.
-                apply q in comp4; clear q; auto.
+                allsimpl; cpx.
+                eapply q in comp4; clear q; auto; try (exact diff);
+                try (complete (apply hasvalue_like_arithop_can_right in hv; auto)).
                 exrepnd.
                 rewrite comp2; auto.
                 eexists; dands; eauto.
-                repeat prove_alpha_eq4.
+                apply diff_abs_bot_alpha_arithop; eauto 3 with slow.
 
               - csunf; simpl.
                 apply isexc_implies2 in comp1; exrepnd; subst.
+                invdiff.
                 dcwf h; simpl; auto.
-                eexists; dands; eauto.
+                eexists; dands; eauto 3 with slow.
             }
 
             {
@@ -886,9 +1612,10 @@ Proof.
               csunf comp; allsimpl.
               apply compute_step_can_test_success in comp.
               repndors; exrepnd; subst; auto.
+              invdiff.
               csunf; simpl.
               eexists; dands; eauto.
-              destruct (canonical_form_test_for c can2); auto.
+              destruct (canonical_form_test_for c can2); eauto 3 with slow.
             }
 
           + SSCase "NCan".
@@ -908,29 +1635,55 @@ Proof.
             autodimp wfn hyp.
             allrw @wf_bterm_iff.
 
-            apply q in Heqc; clear q; auto.
-            exrepnd.
-            csunf; allsimpl.
-            rewrite Heqc1; auto; simpl.
-            eexists; dands; eauto.
-            repeat prove_alpha_eq4.
+            invdiff.
+
+            * applydup @wf_oterm_iff in wf'; repnd.
+              pose proof (wf'0 (bterm [] (oterm (NCan ncan2) bs0))) as wf'n; allsimpl.
+              autodimp wf'n hyp.
+              allrw @wf_bterm_iff.
+
+              apply (q (oterm (NCan ncan2) bs0)) in Heqc; clear q; auto;
+              try (complete (apply hasvalue_like_ncan_fst in hv; auto)).
+              exrepnd.
+              csunf; allsimpl.
+              rewrite Heqc1; auto; simpl.
+              eexists; dands; eauto.
+
+              apply implies_diff_abs_bot_alpha_oterm.
+              apply diff_abs_bot_bs_alpha_cons_if; eauto 3 with slow.
+              apply diff_abs_bot_bterms_implies_diff_abs_bot_bs_alpha.
+              unfold diff_abs_bot_bterms, br_bterms, br_list; dands; auto.
+
+            * apply hasvalue_like_ncan_fst in hv.
+              csunf Heqc; allsimpl; ginv.
+              eapply hasvalue_like_compute_step in hv;
+                [|csunf;simpl;auto].
+              unfold apply_bterm in hv; allsimpl.
+              rewrite lsubst_lsubst_aux in hv; allsimpl; auto.
+              boolvar.
+              apply not_hasvalue_like_vbot in hv; tcsp.
 
           + SSCase "Exc".
 
             csunf comp; allsimpl.
             apply compute_step_catch_success in comp.
-            repndors; exrepnd; subst; allsimpl; ginv.
+            repndors; exrepnd; subst; allsimpl; ginv;
+            invdiff.
 
             * csunf; simpl; auto.
               eexists; dands; eauto.
-              unfold mk_atom_eq.
-              repeat prove_alpha_eq4.
-              eapply alpha_eq_trans;
-                try (apply alpha_eq_sym; apply abs2bot_lsubst); auto.
+              apply diff_abs_bot_alpha_atom_eq; eauto 3 with slow.
+
+              { apply diff_abs_bot_alpha_lsubst; simpl; eauto 3 with slow. }
+
+              { apply diff_abs_bot_alpha_exc; eauto 3 with slow. }
 
             * csunf; simpl; auto.
               rewrite compute_step_catch_if_diff; auto.
               eexists; dands; eauto.
+              apply implies_diff_abs_bot_alpha_oterm.
+              apply diff_abs_bot_bterms_implies_diff_abs_bot_bs_alpha.
+              unfold diff_abs_bot_bterms, br_bterms, br_list; dands; auto.
 
           + SSCase "Abs".
 
@@ -940,109 +1693,113 @@ Proof.
       {
         csunf comp; allsimpl.
         apply compute_step_fresh_success in comp; exrepnd; subst.
-        repndors; exrepnd; subst; ginv.
+        repndors; exrepnd; subst; ginv; invdiff.
 
         - csunf; simpl; boolvar; auto.
-          eexists; dands; eauto.
+          eexists; dands; eauto 3 with slow.
 
         - rewrite compute_step_fresh_if_isvalue_like2; simpl; eauto 3 with slow.
-          eexists; dands; eauto.
-          apply pushdown_fresh_abs2bot; auto.
+          eexists; dands; eauto 3 with slow.
 
         - rewrite compute_step_fresh_if_isnoncan_like; simpl; eauto 3 with slow.
 
           allrw @wf_fresh_iff.
-
-          pose proof (ind t (subst t n (mk_utoken (get_fresh_atom t))) [n]) as q; clear ind.
-          repeat (autodimp q hyp); eauto 2 with slow.
-          { rewrite simple_osize_subst; eauto 2 with slow. }
-          apply q in comp2; clear q; eauto 3 with slow;[].
-          exrepnd; allsimpl.
-
-          pose proof (abs2bot_lsubst t [(n,mk_utoken (get_fresh_atom t))]) as aeq.
-          pose proof (compute_step_alpha
-                        []
-                        (abs2bot (lsubst t [(n, mk_utoken (get_fresh_atom t))]))
-                        (lsubst (abs2bot t) (abs2bot_sub [(n, mk_utoken (get_fresh_atom t))]))
-                        w) as comp.
-          repeat (autodimp comp hyp).
-          { apply implies_nt_wf_abs2bot.
-            apply nt_wf_subst; eauto 2 with slow. }
-          exrepnd; allsimpl.
-          fold_terms; allrw @fold_subst.
-
-          assert (!LIn (get_fresh_atom t) (get_utokens (abs2bot t))) as ni1.
-          {
-            intro h.
-            pose proof (implies_props_abs2bot t) as q; repnd.
-            apply q in h.
-            apply get_fresh_atom_prop in h; tcsp.
-          }
-
-          assert (!LIn (get_fresh_atom (abs2bot t)) (get_utokens (abs2bot t))) as ni2.
-          {
-            intro h.
-            apply get_fresh_atom_prop in h; tcsp.
-          }
-
           pose proof (compute_step_subst_utoken
-                        []
-                        (abs2bot t)
-                        t2'
-                        [(n, mk_utoken (get_fresh_atom t))]) as comp'.
-          repeat (autodimp comp' hyp); simpl; eauto 3 with slow.
-
-          { unfold get_utokens_sub; simpl.
-            apply disjoint_singleton_l; auto. }
-
-          exrepnd; allsimpl.
-
-          pose proof (comp'0 [(n, mk_utoken (get_fresh_atom (abs2bot t)))]) as comp''.
-          allsimpl.
-          repeat (autodimp comp'' hyp); eauto 3 with slow.
-
-          { unfold get_utokens_sub; simpl.
-            apply disjoint_singleton_l; auto. }
-
-          exrepnd; allsimpl.
-          allrw @fold_subst.
-          rewrite comp''1; simpl.
-          eexists; dands; eauto.
-
-          apply implies_alpha_eq_mk_fresh.
-
-          rename comp''0 into aeq1.
-          assert (alpha_eq (subst w0 n (mk_utoken (get_fresh_atom t))) (abs2bot x)) as aeq2.
-          { eauto 4 with slow. }
-
-          unfold get_utokens_sub in *; allsimpl.
+                        [] t x
+                        [(n,mk_utoken (get_fresh_atom t))]) as ch.
+          autorewrite with slow in *; allsimpl.
+          repeat (autodimp ch hyp); eauto 3 with slow;[].
+          exrepnd.
           allrw disjoint_singleton_l.
 
-          eapply alpha_eq_trans;
-            [|apply alpha_eq_sym; apply abs2bot_subst_utokens].
-          simpl.
+          pose proof (fresh_atom o (get_utokens t ++ get_utokens t2)) as fa; exrepnd.
+          allrw in_app_iff; allrw not_over_or; repnd.
+          rename x0 into a.
 
-          eapply alpha_eq_trans;
-            [apply alpha_eq_subst_utokens_same;exact aeq1|].
+          pose proof (ch0 [(n,mk_utoken a)]) as ch'; allsimpl; clear ch0.
+          autorewrite with slow in *; allsimpl.
+          repeat (autodimp ch' hyp); eauto 3 with slow;[]; exrepnd.
 
-          eapply alpha_eq_trans;
-            [apply simple_alphaeq_subst_utokens_subst;
-              intro i; apply comp'4 in i; auto|].
+          pose proof (hasvalue_like_fresh_implies [] a n t) as hv1.
+          repeat (autodimp hv1 hyp).
+          { eapply hasvalue_like_if_compute_step;
+            [|rewrite computation2.compute_step_fresh_if_isnoncan_like;
+               simpl; auto; rewrite comp2;simpl;reflexivity].
+            auto. }
+          applydup @hasvalue_like_compute_step in ch'1 as hv2; auto;[].
 
-          eapply alpha_eq_trans;
-            [|apply alpha_eq_subst_utokens_same;exact aeq2].
+          pose proof (ind t (subst t n (mk_utoken a)) [n]) as q; clear ind.
+          repeat (autodimp q hyp); eauto 2 with slow.
+          { rewrite simple_osize_subst; eauto 2 with slow. }
 
-          eapply alpha_eq_trans;
+          applydup (q (subst t2 n (mk_utoken a))) in ch'1 as comp'; clear q; eauto 4 with slow;
+          [|repeat unfsubst; apply diff_abs_bot_lsubst_aux; simpl; eauto 3 with slow].
+          exrepnd; allsimpl.
+
+          pose proof (compute_step_subst_utoken [] t2 u' [(n,mk_utoken a)]) as ch''.
+          autorewrite with slow in *; allsimpl.
+          repeat (autodimp ch'' hyp); eauto 3 with slow.
+          exrepnd.
+
+          pose proof (ch''0 [(n,mk_utoken (get_fresh_atom t2))]) as ch'''; clear ch''0.
+          autorewrite with slow in *; allsimpl.
+          repeat (autodimp ch''' hyp); eauto 3 with slow.
+          exrepnd.
+
+          allrw @fold_subst.
+          rewrite ch'''1; simpl.
+          eexists; dands; eauto.
+          apply diff_abs_bot_alpha_fresh.
+
+          assert (!LIn (get_fresh_atom t2) (get_utokens w0)) as ni1.
+          {
+            intro i.
+            apply ch''4 in i.
+            apply get_fresh_atom_prop in i; tcsp.
+          }
+
+          assert (!LIn a (get_utokens w)) as ni2.
+          {
+            intro i.
+            apply ch4 in i; auto.
+          }
+
+          assert (!LIn a (get_utokens w0)) as ni3.
+          {
+            intro i.
+            apply ch''4 in i; auto.
+          }
+
+          eapply diff_abs_bot_alpha_l;
+            [apply alpha_eq_subst_utokens_same;exact ch1|].
+          eapply diff_abs_bot_alpha_r;
+            [|apply alpha_eq_sym;apply alpha_eq_subst_utokens_same;exact ch'''0].
+
+          eapply diff_abs_bot_alpha_l;
+            [apply simple_alphaeq_subst_utokens_subst;auto|].
+          eapply diff_abs_bot_alpha_r;
             [|apply alpha_eq_sym;apply simple_alphaeq_subst_utokens_subst;auto].
 
-          auto.
+          pose proof (simple_alphaeq_subst_utokens_subst w n a) as aeq1.
+          autodimp aeq1 hyp.
+          pose proof (simple_alphaeq_subst_utokens_subst w0 n a) as aeq2.
+          autodimp aeq2 hyp.
+          eapply diff_abs_bot_alpha_l;[apply alpha_eq_sym;exact aeq1|].
+          eapply diff_abs_bot_alpha_r;[|exact aeq2].
+          eapply diff_abs_bot_alpha_l;
+            [apply alpha_eq_sym;apply alpha_eq_subst_utokens_same;exact ch'0|].
+          eapply diff_abs_bot_alpha_r;
+            [|apply alpha_eq_subst_utokens_same;exact ch''1].
+          apply diff_abs_bot_alpha_subst_utokens.
+          eauto 3 with slow.
       }
 
     + SCase "Exc".
 
       csunf comp; allsimpl; ginv.
+      invdiff.
       csunf; simpl.
-      eexists; dands; eauto.
+      eexists; dands; eauto 3 with slow.
 
     + SCase "Abs".
 
